Adding the random oracle treatment

hol/p4_concurrency_testLib.sig
@@ -1,0 +1,8 @@
+signature p4_concurrency_testLib =
+sig
+  include Abbrev
+
+val get_trace_thread_n : string -> term -> term -> int -> int -> thm
+val get_trace_thread_next_n : string -> term -> thm -> int -> int -> thm
+
+end
